Add tests for programs that return HO arrows

io/Compile.RILang.To.MLang.fst
@@ -41,6 +41,24 @@ instance compilable_int pi : compilable int pi = {
   compile = (fun x -> x);
 }
 
+instance compilable_int_arrow
+  pi
+  (t2:Type) {| d2:compilable t2 pi |} :
+  Tot (compilable (int -> rilang_dm pi t2) pi) = {
+  rilang_comp_in = rilang_arrow pi (rilang_int pi) d2.rilang_comp_in;
+
+  comp_out = int -> free.m d2.comp_out;
+  mlang_comp_out = mlang_free_arrow mlang_int d2.mlang_comp_out;
+
+  compile = (fun (f:(int -> rilang_dm pi t2)) (tgt_x:int) ->
+    let src_x : int = tgt_x in
+    let r : rilang_dm pi t2 = f src_x in
+    let r = as_iio_dm r in 
+    let w = IIO.dm_iio_bind _ _ _ (fun _ -> (pi_as_hist pi)) r (fun x -> IIO.dm_iio_return _ (d2.compile x)) in
+    w
+  );
+}
+
 (** *** Compilable arrows **)
 instance compilable_arrow
   pi
@@ -64,7 +82,7 @@ instance compilable_arrow
 
 (** ** Manual testing *)
 (* TODO:
-  - [ ] support HO on the return type
+  - [v] support HO on the return type
   - [ ] support different pi for the ctx
 *)
 noeq
@@ -75,14 +93,14 @@ type interface = {
   rilang_ct  : rilang (ct (dm_mon vpi).m) vpi;
   mlang_ct   : mlang (ct free.m);
 
-  //pt:(Type->Type)->Type0;
-  //compilable_pt : compilable (pt (dm_mon vpi).m) vpi;
+  pt:(Type->Type)->Type;
+  compilable_pt : compilable (pt (dm_mon vpi).m) vpi;
 }
 
 
 type ictx (i:interface) (ipi:monitorable_prop) = i.ct (dm_mon ipi).m
-type iprog (i:interface)  = ictx i i.vpi -> rilang_dm i.vpi int
-type iwhole (i:interface) = unit -> rilang_dm i.vpi int 
+type iprog (i:interface)  = ictx i i.vpi -> rilang_dm i.vpi (i.pt (dm_mon i.vpi).m)
+type iwhole (i:interface) = unit -> rilang_dm i.vpi (i.pt (dm_mon i.vpi).m) 
 
 type r_vpi_ipi (vpi ipi:monitorable_prop) = squash (forall h lt. enforced_locally ipi h lt ==> enforced_locally vpi h lt)
 
@@ -97,8 +115,8 @@ let ilink
 
 (** *** Target Lang **)
 type ctx (i:interface) = mon:monad -> acts mon -> i.ct mon.m
-type prog (i:interface) = ctx i -> free.m int 
-type whole (i:interface) = unit -> free.m int 
+type prog (i:interface) = ctx i -> free.m i.compilable_pt.comp_out
+type whole (i:interface) = unit -> free.m i.compilable_pt.comp_out 
 let link (#i:interface) (p:prog i) (c:ctx i) : whole i = fun () -> p c
 
 #reset-options
@@ -107,14 +125,13 @@ let prog_compilable (i:interface) : compilable (iprog i) i.vpi =
   compilable_arrow
     i.vpi
     i.ct #i.rilang_ct #i.mlang_ct
-    int #(compilable_int i.vpi)
+    (i.pt (dm_mon i.vpi).m) #i.compilable_pt
 
 let model_compile
   (#i:interface)
   (ip:iprog i) :
   prog i = 
-  let p : (prog_compilable i).comp_out = (prog_compilable i).compile ip in
-  p
+  (prog_compilable i).compile ip
 
 (** *** Case Studies **)
 
@@ -124,9 +141,11 @@ let test1 : interface = {
   vpi = thePi;
 
   ct = (fun m -> (int -> m int));
-
   rilang_ct = rilang_arrow thePi (rilang_int thePi) (rilang_int thePi);
   mlang_ct = mlang_free_arrow mlang_int mlang_int;
+
+  pt = (fun m -> int);
+  compilable_pt = compilable_int thePi;
 }
 
 let iprog1 : iprog test1 = fun c -> (dm_mon thePi).bind (c 5) (fun r -> (dm_mon thePi).ret (r + 1))
@@ -142,10 +161,12 @@ let mwhole1 = mprog1 `link` mctx1
 let test2 : interface = {
   vpi = thePi;
 
-  (* intermediate level *)
   ct = (fun m -> (int -> m int) -> m int);
   rilang_ct = rilang_arrow thePi (rilang_arrow thePi (rilang_int thePi) (rilang_int thePi)) (rilang_int thePi);
   mlang_ct = mlang_free_arrow (mlang_free_arrow mlang_int mlang_int) mlang_int;
+
+  pt = (fun m -> int);
+  compilable_pt = compilable_int thePi;
 }
 
 let iprog2 : iprog test2 = fun c -> (dm_mon thePi).bind (c (fun x -> (dm_mon thePi).ret (x + 5))) (fun r -> (dm_mon thePi).ret (r + 1))
@@ -154,3 +175,51 @@ val mctx2 : ctx test2
 let mctx2 (mon:monad) (acts:acts mon) (f:int -> mon.m int) : mon.m int =
   mon.bind (f 5) (fun x -> mon.ret (x+2))
 let mwhole2 = mprog2 `link` mctx2
+
+let test3 : interface = {
+  vpi = thePi;
+
+  ct = (fun m -> (int -> m int) -> m int);
+  rilang_ct = rilang_arrow thePi (rilang_arrow thePi (rilang_int thePi) (rilang_int thePi)) (rilang_int thePi);
+  mlang_ct = mlang_free_arrow (mlang_free_arrow mlang_int mlang_int) mlang_int;
+
+  pt = (fun m -> int -> m int);
+  compilable_pt = compilable_int_arrow thePi int #(compilable_int thePi);
+}
+
+let test4 : interface = {
+  vpi = thePi;
+
+  ct = (fun m -> (int -> m int) -> m int);
+  rilang_ct = rilang_arrow thePi (rilang_arrow thePi (rilang_int thePi) (rilang_int thePi)) (rilang_int thePi);
+  mlang_ct = mlang_free_arrow (mlang_free_arrow mlang_int mlang_int) mlang_int;
+
+  pt = (fun m -> (int -> m int) -> m int);
+  compilable_pt = compilable_arrow thePi (fun m -> int -> m int) #(rilang_arrow thePi (rilang_int thePi) (rilang_int thePi)) #(mlang_free_arrow mlang_int mlang_int) int #(compilable_int thePi);
+}
+
+
+val iprog4 : iprog test4
+let iprog4 ctx = (dm_mon thePi).ret (fun cb -> cb 5)
+let mprog4 : prog test4 = model_compile iprog4 //thePi
+val mctx4 : ctx test4  
+let mctx4 (mon:monad) (acts:acts mon) (f:int -> mon.m int) : mon.m int =
+  mon.bind (f 5) (fun x -> mon.ret (x+2))
+
+let mwhole4 = mprog4 `link` mctx4
+
+let _ = assert (has_type mwhole4 (unit -> free.m (test4.compilable_pt.comp_out))) by (norm [delta_only [`%Mkcompilable?.comp_out;`%Mkinterface?.compilable_pt;`%Mkmonad?.m;`%Mkinterface?.pt]; iota;zeta]; dump "H")
+
+let _ = assert (test4.compilable_pt.comp_out == ((mon:monad -> acts mon -> (int -> mon.m int)) -> free.m int)) by (compute ())
+
+let mwhole4' : (unit -> free.m ((mon:monad -> acts mon -> (int -> mon.m int)) -> free.m int)) =
+  assert (has_type mwhole4 (unit -> free.m ((mon:monad -> acts mon -> (int -> mon.m int)) -> free.m int))) by (compute ());
+  admit ();
+  mwhole4
+  
+(* TODO: probably can not bind because the types are not in the same universe *)
+let _ = 
+  let whole4 : free.m ((mon:monad -> acts mon -> (int -> mon.m int)) -> free.m int) = mwhole4' () in
+  free.bind whole4 #((mon:monad -> acts mon -> (int -> mon.m int)) -> free.m int) #int (fun (p:((mon:monad -> acts mon -> (int -> mon.m int)) -> free.m int)) ->
+    let r : free.m int = p mctx1 in
+    r)
